\documentclass[]{article}
\usepackage{amsmath}
\usepackage{amssymb}
\usepackage{amsfonts}
\usepackage{mathtools}
\usepackage
[
left=2cm,
right=2cm,
top=2cm,
bottom=2cm,
]
{geometry}

\newcommand{\ud}{\mathrm{d}}

\title{Sierpinski Expression}

\begin{document}
\maketitle
If we have recursive function 
\begin{align*}
f_0^{a,b,u,v}(x, y) &= ax + by\\
f_{n+1}^{a,b,u,v} (x, y) &= f_n^{a,b,u,v}(f_n^{a,b,u,v}(x, u), f_n^{a,b,u,v}(v, y))\,,
\end{align*}
then we have
\begin{align*}
f_n^{a,b,u,v}(x, y) &= a^{2^n}x + b^{2^n}y + \frac{u+v}{2}\left( 1 - a^{2^n} - b^{2^n} + (a+b - 1)  \prod_{k=0}^{n-1}(a^{2^k}+b^{2^k}+1) \right)\\
f_\infty^{a,b,u,v} &=\frac{u+v}{2}\left( 1 + (a+b - 1) \prod_{k=0}^{\infty}(a^{2^k}+b^{2^k}+1)\right)
\end{align*}

Proof by induction:
\begin{align*}
f_0^{a,b,u,v}(x, y) &=  a^{2^0}x + b^{2^0}y + \frac{u+v}{2}\left( 1 - a^{2^0} - b^{2^0} + (a+b - 1)  \prod_{k=0}^{-1}(a^{2^k}+b^{2^k}+1) \right) \\
 &= ax + by + \frac{u+v}{2}\left( 1 - a - b + (a+b - 1)  \right) \\
 &= ax + by
\end{align*}

\begin{align*}
f_{n+1}^{a,b,u,v} (x, y) &= f_n^{a,b,u,v}(f_n^{a,b,u,v}(x, u), f_n^{a,b,u,v}(v, y)) \\
&= a^{2^n}\left(a^{2^n}x + b^{2^n}u + \frac{u+v}{2}\left( 1 - a^{2^n} - b^{2^n} + (a+b - 1)  \prod_{k=0}^{n-1}(a^{2^k}+b^{2^k}+1) \right)\right) \\ &+ b^{2^n}\left(a^{2^n}v + b^{2^n}y + \frac{u+v}{2}\left( 1 - a^{2^n} - b^{2^n} + (a+b - 1)  \prod_{k=0}^{n-1}(a^{2^k}+b^{2^k}+1) \right)\right) \\ &+ \frac{u+v}{2}\left( 1 - a^{2^n} - b^{2^n} + (a+b - 1)  \prod_{k=0}^{n-1}(a^{2^k}+b^{2^k}+1) \right)\\
&= a^{2^{n+1}} x +b^{2^{n+1}} y + a^{2^{n}}b^{2^{n}}(u+v) + \frac{u+v}{2}(a^{2^n} + b^{2^n} + 1)\left( 1 - a^{2^n} - b^{2^n} + (a+b - 1)  \prod_{k=0}^{n-1}(a^{2^k}+b^{2^k}+1) \right) \\
&= a^{2^{n+1}} x +b^{2^{n+1}} y + a^{2^{n}}b^{2^{n}}(u+v) + \frac{u+v}{2}\left( 1 - a^{2^{n+1}} - b^{2^{n+1}} - 2a^{2^n}b^{2^n} + (a+b - 1)  \prod_{k=0}^{n}(a^{2^k}+b^{2^k}+1) \right) \\
&= a^{2^{n+1}} x +b^{2^{n+1}} y  + \frac{u+v}{2}\left( 1 - a^{2^{n+1}} - b^{2^{n+1}} + (a+b - 1)  \prod_{k=0}^{n}(a^{2^k}+b^{2^k}+1) \right) \\
\end{align*}
 
\end{document}